src/Basic.v
@@ -1,0 +1,144 @@
+Require Import PArith.
+Require Import ZArith.
+Require Import FunctionalExtensionality.
+Require Import ClassicalFacts.
+Require Import Relations.
+Require Import RelationClasses.
+Require Import EquivDec.
+Require Import List.
+Require Import SetoidList.
+Require Import sflib.
+
+Set Implicit Arguments.
+
+
+Ltac refl := reflexivity.
+Ltac congr := congruence.
+Ltac etrans := etransitivity.
+Ltac etrans' :=
+  match goal with
+  | [H: @PreOrder ?A ?R |- ?R (_:?A) (_:?A)] =>
+    eapply (@PreOrder_Transitive _ _ H)
+  end.
+Ltac antisym :=
+  match goal with
+  | [H: @PartialOrder ?A ?EQ _ ?LE _ |- ?EQ (_:?A) (_:?A)] =>
+    apply (partial_order_antisym H)
+  end.
+Ltac funext := apply functional_extensionality.
+Axiom propext: prop_extensionality.
+Ltac propext := apply propext.
+
+Ltac condtac :=
+  match goal with
+  | [|- context[if ?c then _ else _]] =>
+    let X := fresh "X" in
+    destruct c eqn:X
+  end.
+
+Definition proj_sumbool (P Q: Prop) (a: {P} + {Q}) : bool :=
+  if a then true else false.
+Arguments proj_sumbool [P Q].
+Coercion proj_sumbool: sumbool >-> bool.
+
+Notation rtc := (clos_refl_trans_1n _). (* reflexive transitive closure *)
+Notation rc := (clos_refl _). (* reflexive transitive closure *)
+Notation tc := (clos_trans_1n _). (* transitive closure *)
+Hint Immediate rt1n_refl rt1n_trans t1n_step.
+Hint Resolve Relation_Operators.rt1n_trans.
+
+Program Instance rtc_PreOrder A (R:A -> A -> Prop): PreOrder (rtc R).
+Next Obligation.
+  ii. revert H0. induction H; auto. i.
+  exploit IHclos_refl_trans_1n; eauto.
+Qed.
+
+Lemma rtc_step_tc
+      A a b c
+      (rel:relation A)
+      (AB: rtc rel a b)
+      (BC: rel b c):
+  tc rel a c.
+Proof.
+  revert c BC. induction AB.
+  - i. econs. ss.
+  - i. exploit IHAB; eauto. i.
+    eapply Relation_Operators.t1n_trans; eauto.
+Qed.
+
+Fixpoint filter_map A B (f: A -> option B) (l: list A): list B :=
+  match l with
+  | [] => []
+  | a::l =>
+    match f a with
+    | None => filter_map f l
+    | Some b => b :: filter_map f l
+    end
+  end.
+
+Lemma in_filter_map_iff A B (f: A -> option B) (l: list A) (b: B):
+  List.In b (filter_map f l) <-> exists a, List.In a l /\ f a = Some b.
+Proof.
+  induction l; ss.
+  { econs; i; des; ss. }
+  destruct (f a) eqn:FA; ss.
+  - rewrite IHl. intuition; des; subst; eauto.
+    rewrite FA in H2. inv H2. auto.
+  - rewrite IHl. intuition; des; subst; eauto. congr.
+Qed.
+
+Lemma SetoidList_findA_rev
+      (A B : Type) (eqA : A -> A -> Prop)
+      (EQUIV: Equivalence eqA)
+      (eqA_dec : forall x y : A, {eqA x y} + {~ eqA x y})
+      (l : list (A * B))
+      (a : A) (b : B)
+      (NODUP: SetoidList.NoDupA (fun p p' : A * B => eqA (fst p) (fst p')) l):
+  SetoidList.findA (fun a' : A => if eqA_dec a a' then true else false) l =
+  SetoidList.findA (fun a' : A => if eqA_dec a a' then true else false) (List.rev l).
+Proof.
+  hexploit SetoidList.NoDupA_rev; try exact NODUP; [|i].
+  { econs; ii.
+    - refl.
+    - symmetry. ss.
+    - etrans; eauto.
+  }
+
+  match goal with
+  | [|- ?f = _] => destruct f eqn:FIND
+  end.
+  { rewrite <- SetoidList.findA_NoDupA in FIND; ss.
+    rewrite <- SetoidList.InA_rev in FIND.
+    rewrite SetoidList.findA_NoDupA in FIND; ss.
+    eauto.
+  }
+
+  match goal with
+  | [|- _ = ?f] => destruct f eqn:FIND'
+  end.
+  { rewrite <- SetoidList.findA_NoDupA in FIND'; ss.
+    rewrite SetoidList.InA_rev in FIND'.
+    rewrite SetoidList.findA_NoDupA in FIND'; ss.
+    rewrite FIND' in FIND. congr.
+  }
+
+  ss.
+Qed.
+
+Inductive opt_pred A (pred: A -> Prop): forall (a:option A), Prop :=
+| opt_pred_intro
+    a
+    (PRED: pred a):
+    opt_pred pred (Some a)
+.
+Hint Constructors opt_pred.
+
+Inductive opt_rel A B (rel: A -> B -> Prop): forall (a:option A) (b:option B), Prop :=
+| opt_rel_None:
+    opt_rel rel None None
+| opt_rel_Some
+    a b
+    (REL: rel a b):
+    opt_rel rel (Some a) (Some b)
+.
+Hint Constructors opt_rel.
