src/HahnRelationsMore.v
@@ -1,0 +1,136 @@
+Require Import sflib.
+Require Import HahnRelationsBasic.
+
+Require Import Basic.
+Require Import Order.
+
+Set Implicit Arguments.
+
+
+Lemma seq_assoc A (r1 r2 r3:relation A):
+  r1 ⨾ (r2 ⨾ r3) = (r1 ⨾ r2) ⨾ r3.
+Proof.
+  funext. i. funext. i. propext. econs; i.
+  - inv H. des. inv H1. des. repeat econs; eauto.
+  - inv H. des. inv H0. des. repeat econs; eauto.
+Qed.
+
+Lemma seq_union A (r1 r2 r3:relation A):
+  r1 ⨾ (r2 ∪ r3) = (r1 ⨾ r2) ∪ (r1 ⨾ r3).
+Proof.
+  funext. i. funext. i. propext. econs; i.
+  - inv H. des. inv H1.
+    + left. econs; eauto.
+    + right. econs; eauto.
+  - inv H; inv H0; des.
+    + econs; esplits; eauto. left. ss.
+    + econs; esplits; eauto. right. ss.
+Qed.
+
+Lemma seq_union' A (r2 r3 r1:relation A):
+  r1 ⨾ (r2 ∪ r3) = (r1 ⨾ r2) ∪ (r1 ⨾ r3).
+Proof.
+  apply seq_union.
+Qed.
+
+Lemma union_seq A (r1 r2 r3:relation A):
+  (r1 ∪ r2) ⨾ r3 = (r1 ⨾ r3) ∪ (r2 ⨾ r3).
+Proof.
+  funext. i. funext. i. propext. econs; i.
+  - inv H. des. inv H0.
+    + left. econs; eauto.
+    + right. econs; eauto.
+  - inv H; inv H0; des.
+    + econs; esplits; eauto. left. ss.
+    + econs; esplits; eauto. right. ss.
+Qed.
+
+Lemma union_seq' A (r3 r1 r2:relation A):
+  (r1 ∪ r2) ⨾ r3 = (r1 ⨾ r3) ∪ (r2 ⨾ r3).
+Proof.
+  apply union_seq.
+Qed.
+
+Lemma clos_refl_union
+      A (r:relation A):
+  r^? = r ∪ eq.
+Proof.
+  funext. i. funext. i. propext. econs; i.
+  - inv H; [right|left]; ss.
+  - inv H; [right|left]; ss.
+Qed.
+
+Lemma eq_seq
+      A (r:relation A):
+  eq ⨾ r = r.
+Proof.
+  funext. i. funext. i. propext. econs; i.
+  - inv H. des. subst. ss.
+  - econs; eauto.
+Qed.
+
+Lemma union_assoc A (r1 r2 r3: relation A):
+  r1 ∪ (r2 ∪ r3) = (r1 ∪ r2) ∪ r3.
+Proof.
+  funext. i. funext. i. propext. econs; i.
+  - inv H; [|inv H0].
+    + left. left. ss.
+    + left. right. ss.
+    + right. ss.
+  - inv H; [inv H0|].
+    + left. ss.
+    + right. left. ss.
+    + right. right. ss.
+Qed.
+
+Lemma union_l
+      A
+      (r1 r2: relation A)
+      a b
+      (R1: r1 a b):
+  (r1 ∪ r2) a b.
+Proof. left. ss. Qed.
+
+Lemma union_r
+      A
+      (r1 r2: relation A)
+      a b
+      (R2: r2 a b):
+  (r1 ∪ r2) a b.
+Proof. right. ss. Qed.
+
+Lemma cross_bot_l
+      A (pred:A -> Prop):
+  bot × pred = bot.
+Proof.
+  funext. i. funext. i. propext.
+  econs; intro X; inv X. inv H.
+Qed.
+
+Lemma cross_bot_r
+      A (pred:A -> Prop):
+  pred × bot = bot.
+Proof.
+  funext. i. funext. i. propext.
+  econs; intro X; inv X. inv H0.
+Qed.
+
+Lemma union_bot_l
+      A (rel: relation A):
+  bot ∪ rel = rel.
+Proof.
+  funext. i. funext. i. propext.
+  econs; intro X.
+  - inv X; ss.
+  - right. ss.
+Qed.
+
+Lemma union_bot_r
+      A (rel: relation A):
+  rel ∪ bot = rel.
+Proof.
+  funext. i. funext. i. propext.
+  econs; intro X.
+  - inv X; ss.
+  - left. ss.
+Qed.
