src/Memory.v
@@ -7,6 +7,7 @@ Require Import FSetPositive.
 Require Import EquivDec.
 Require Import sflib.
 
+Require Import Basic.
 Require Import Order.
 Require Import Time.
 Require Import Lang.
