src/Order.v
@@ -8,49 +8,9 @@ Require Import EquivDec.
 Require Import List.
 Require Import sflib.
 
+Require Import Basic.
+
 Set Implicit Arguments.
-
-
-Ltac refl := reflexivity.
-Ltac congr := congruence.
-Ltac etrans := etransitivity.
-Ltac etrans' :=
-  match goal with
-  | [H: @PreOrder ?A ?R |- ?R (_:?A) (_:?A)] =>
-    eapply (@PreOrder_Transitive _ _ H)
-  end.
-Ltac antisym :=
-  match goal with
-  | [H: @PartialOrder ?A ?EQ _ ?LE _ |- ?EQ (_:?A) (_:?A)] =>
-    apply (partial_order_antisym H)
-  end.
-Ltac funext := apply functional_extensionality.
-Axiom propext: prop_extensionality.
-Ltac propext := apply propext.
-
-Ltac condtac :=
-  match goal with
-  | [|- context[if ?c then _ else _]] =>
-    let X := fresh "X" in
-    destruct c eqn:X
-  end.
-
-Definition proj_sumbool (P Q: Prop) (a: {P} + {Q}) : bool :=
-  if a then true else false.
-Arguments proj_sumbool [P Q].
-Coercion proj_sumbool: sumbool >-> bool.
-
-Notation rtc := (clos_refl_trans_1n _). (* reflexive transitive closure *)
-Notation rc := (clos_refl _). (* reflexive transitive closure *)
-Notation tc := (clos_trans_1n _). (* transitive closure *)
-Hint Immediate rt1n_refl rt1n_trans t1n_step.
-Hint Resolve Relation_Operators.rt1n_trans.
-
-Program Instance rtc_PreOrder A (R:A -> A -> Prop): PreOrder (rtc R).
-Next Obligation.
-  ii. revert H0. induction H; auto. i.
-  exploit IHclos_refl_trans_1n; eauto.
-Qed.
 
 
 Class orderC (A:Type) (EQ LE: relation A) (join: forall (a b:A), A) (bot: A) `{_: PartialOrder A EQ LE} := mk {
