src/Time.v
@@ -5,6 +5,7 @@ Require Import Lia.
 Require Import EquivDec.
 Require Import sflib.
 
+Require Import Basic.
 Require Import Order.
 
 Set Implicit Arguments.
